formal/coq/extraction/ExtractTransitionVectors.v
@@ -36,6 +36,7 @@ Extraction "transition_extracted.ml"
   TransitionExtraction.extract_apply_block_transitions_structural
   TransitionExtraction.extract_apply_valid_block_structural
   TransitionExtraction.extract_utxo_domain
+  TransitionExtraction.extract_utxo_total_value
   TransitionExtraction.extract_domain_has_no_duplicates
   TransitionExtraction.extract_domain_below_bool
   TransitionExtraction.extract_block_output_count
